making the two example layered effects reifiable and reflectable, and adding example of an action added via reflect

examples/layeredeffects/HoareST.fst
@@ -89,9 +89,24 @@ let conjunction (a:Type)
 
 /// Actions
 
+/// We define read action with the effect, but write will be defined via reflect later
+
 let read (a:Type0) (r:ref a)
 : repr a (fun _ -> True) (fun h0 x h1 -> h0 == h1 /\ x == sel h0 r)
 = fun _ -> read r 
+
+reifiable reflectable
+layered_effect {
+  HoareST : a:Type -> pre:pre_t -> post:post_t a -> Effect
+  with repr        = repr;
+       return      = return;
+       bind        = bind;
+       stronger    = stronger;
+       conjunction = conjunction;
+
+       read = read
+}
+
 
 let write (a:Type0) (r:ref a) (x:a)
 : repr unit
@@ -102,39 +117,27 @@ let write (a:Type0) (r:ref a) (x:a)
     sel h1 r == x)
 = fun _ -> write r x
 
-layered_effect {
-  HoareST : a:Type -> pre:pre_t -> post:post_t a -> Effect
-  with repr        = repr;
-       return      = return;
-       bind        = bind;
-       stronger    = stronger;
-       conjunction = conjunction;
-
-       read = read;
-       write = write
-}
-
 let mread = HoareST?.read
-let mwrite = HoareST?.write
+let mwrite (a:Type0) (r:ref a) (x:a) = HoareST?.reflect (write a r x)
 
-assume val wp_monotonic_pure (_:unit)
-  : Lemma
-    (forall (a:Type) (wp:pure_wp a).
-       (forall (p q:pure_post a).
-          (forall (x:a). p x ==> q x) ==>
-          (wp p ==> wp q)))
+// assume val wp_monotonic_pure (_:unit)
+//   : Lemma
+//     (forall (a:Type) (wp:pure_wp a).
+//        (forall (p q:pure_post a).
+//           (forall (x:a). p x ==> q x) ==>
+//           (wp p ==> wp q)))
 
-/// lift from PURE
+// /// lift from PURE
 
-let lift_pure_hoarest (a:Type) (wp:pure_wp a) (f:unit -> PURE a wp)
-: repr a
-  (fun _ -> wp (fun _ -> True))
-  (fun h0 r h1 -> ~ (wp (fun x -> x =!= r \/ h0 =!= h1)))
-= wp_monotonic_pure ();
-  fun _ ->
-  f ()
+// let lift_pure_hoarest (a:Type) (wp:pure_wp a) (f:unit -> PURE a wp)
+// : repr a
+//   (fun _ -> wp (fun _ -> True))
+//   (fun h0 r h1 -> ~ (wp (fun x -> x =!= r \/ h0 =!= h1)))
+// = wp_monotonic_pure ();
+//   fun _ ->
+//   f ()
 
-sub_effect PURE ~> HoareST = lift_pure_hoarest
+// sub_effect PURE ~> HoareST = lift_pure_hoarest
 
 // type repr (a:Type) (n:nat) (wp:pure_wp a) = unit -> PURE a wp
 
